coq/NRAEnv/Extended/NRAEnv.v
@@ -216,27 +216,6 @@ Section NRAEnv.
     reflexivity.
   Qed.
 
-  Section size.
-    Require Import RAlgEnvSize.
-    Definition nraenv_size (q:nraenv) :=
-      algenv_size (algenv_of_nraenv q).
-    Definition nraenv_depth (q:nraenv) :=
-      algenv_depth (algenv_of_nraenv q).
-  End size.
-
-  Section ignore.
-    Require Import RAlgEnvIgnore.
-    Definition nraenv_ignores_id (q:nraenv) :=
-      ignores_id (algenv_of_nraenv q).
-    Definition nraenv_ignores_id_fun (q:nraenv) :=
-      ignores_id_fun (algenv_of_nraenv q).
-
-    Definition nraenv_ignores_env (q:nraenv) :=
-      ignores_env (algenv_of_nraenv q).
-    Definition nraenv_ignores_env_fun (q:nraenv) :=
-      ignores_env_fun (algenv_of_nraenv q).
-  End ignore.
-
   Section dup.
     Require Import ROptimEnv.
     (* optimization for distinct *)
