coq/NRAEnv/Extended/NRAEnvIgnore.v
@@ -1,0 +1,400 @@
+(*
+ * Copyright 2015-2016 IBM Corporation
+ *
+ * Licensed under the Apache License, Version 2.0 (the "License");
+ * you may not use this file except in compliance with the License.
+ * You may obtain a copy of the License at
+ *
+ * http://www.apache.org/licenses/LICENSE-2.0
+ *
+ * Unless required by applicable law or agreed to in writing, software
+ * distributed under the License is distributed on an "AS IS" BASIS,
+ * WITHOUT WARRANTIES OR CONDITIONS OF ANY KIND, either express or implied.
+ * See the License for the specific language governing permissions and
+ * limitations under the License.
+ *)
+
+Section NRAEnvIgnore.
+
+  Require Import Bool List String.
+  Require Import Utils BasicRuntime.
+  Require Import NRAEnv.
+
+  (* Some of algebraic equivalences for NRA with environment *)
+  (* Those are valid without type *)
+
+  Local Open Scope alg_scope.
+  Local Open Scope nraenv_scope.
+  
+  (** Some infrastructure for rewrites *)
+
+  Context {fruntime:foreign_runtime}.
+
+  Fixpoint is_nra (e:nraenv) : Prop :=
+    match e with
+      | NRAEnvID => True
+      | NRAEnvConst rd => True
+      | NRAEnvBinop bop e1 e2 => (is_nra e1) /\ (is_nra e2)
+      | NRAEnvUnop uop e1 => is_nra e1
+      | NRAEnvMap e1 e2 => (is_nra e1) /\ (is_nra e2)
+      | NRAEnvMapConcat e1 e2 => (is_nra e1) /\ (is_nra e2)
+      | NRAEnvProduct e1 e2 => (is_nra e1) /\ (is_nra e2)
+      | NRAEnvSelect e1 e2 => (is_nra e1) /\ (is_nra e2)
+      | NRAEnvDefault e1 e2 => (is_nra e1) /\ (is_nra e2)
+      | NRAEnvEither e1 e2 => (is_nra e1) /\ (is_nra e2)
+      | NRAEnvEitherConcat e1 e2 => (is_nra e1) /\ (is_nra e2)
+      | NRAEnvApp e1 e2 => (is_nra e1) /\ (is_nra e2)
+      | NRAEnvGetConstant _ => False
+      | NRAEnvEnv => False
+      | NRAEnvAppEnv e1 e2 => False
+      | NRAEnvMapEnv e1 => False
+      (* Those are additional operators *)
+      | NRAEnvFlatMap e1 e2 => (is_nra e1) /\ (is_nra e2)
+      | NRAEnvJoin e1 e2 e3 =>  (is_nra e1) /\ (is_nra e2) /\ (is_nra e3)
+      | NRAEnvProject _ e1 => (is_nra e1)
+      | NRAEnvGroupBy _ _ e1 => (is_nra e1)
+    end.
+
+  Fixpoint is_nra_fun (e:nraenv) : bool :=
+    match e with
+      | NRAEnvID => true
+      | NRAEnvConst rd => true
+      | NRAEnvBinop bop e1 e2 => andb (is_nra_fun e1) (is_nra_fun e2)
+      | NRAEnvUnop uop e1 => is_nra_fun e1
+      | NRAEnvMap e1 e2 => andb (is_nra_fun e1) (is_nra_fun e2)
+      | NRAEnvMapConcat e1 e2 => andb (is_nra_fun e1) (is_nra_fun e2)
+      | NRAEnvProduct e1 e2 => andb (is_nra_fun e1) (is_nra_fun e2)
+      | NRAEnvSelect e1 e2 => andb (is_nra_fun e1) (is_nra_fun e2)
+      | NRAEnvDefault e1 e2 => andb (is_nra_fun e1) (is_nra_fun e2)
+      | NRAEnvEither e1 e2 => andb (is_nra_fun e1) (is_nra_fun e2)
+      | NRAEnvEitherConcat e1 e2 => andb (is_nra_fun e1) (is_nra_fun e2)
+      | NRAEnvApp e1 e2 => andb (is_nra_fun e1) (is_nra_fun e2)
+      | NRAEnvGetConstant _ => false
+      | NRAEnvEnv => false
+      | NRAEnvAppEnv e1 e2 => false
+      | NRAEnvMapEnv e1 => false
+      (* Those are additional operators *)
+      | NRAEnvFlatMap e1 e2 => andb (is_nra_fun e1) (is_nra_fun e2)
+      | NRAEnvJoin e1 e2 e3 =>  andb (is_nra_fun e1) (andb (is_nra_fun e2) (is_nra_fun e3))
+      | NRAEnvProject _ e1 => (is_nra_fun e1)
+      | NRAEnvGroupBy _ _ e1 => (is_nra_fun e1)
+    end.
+
+  Lemma is_nra_eq (e:nraenv):
+    is_nra e <-> (is_nra_fun e = true).
+  Proof.
+    induction e; split; simpl; intros; try auto; try congruence;
+    try (rewrite IHe1 in H; rewrite IHe2 in H;
+         elim H; clear H; intros;
+         rewrite H; rewrite H0; reflexivity);
+    try (rewrite andb_true_inversion in H;
+         elim H; clear H; intros;
+         rewrite <- IHe1 in H; rewrite <- IHe2 in H0;
+         split; assumption);
+    try (rewrite IHe in H; assumption);
+    try (rewrite <- IHe in H; assumption).
+    - rewrite IHe1 in H; rewrite IHe2 in H; rewrite IHe3 in H.
+      elim H; clear H; intros.
+      elim H0; clear H0; intros.
+      rewrite H; rewrite H0; rewrite H1.
+      auto.
+    - rewrite andb_true_inversion in H.
+      rewrite andb_true_inversion in H.
+      elim H; clear H; intros.
+      elim H0; clear H0; intros.
+      rewrite <- IHe1 in H; rewrite <- IHe2 in H0; rewrite <- IHe3 in H1.
+      auto.
+  Qed.
+
+  Fixpoint nraenv_ignores_env (e:nraenv) : Prop :=
+    match e with
+      | NRAEnvID => True
+      | NRAEnvConst rd => True
+      | NRAEnvBinop bop e1 e2 => (nraenv_ignores_env e1) /\ (nraenv_ignores_env e2)
+      | NRAEnvUnop uop e1 => nraenv_ignores_env e1
+      | NRAEnvMap e1 e2 => (nraenv_ignores_env e1) /\ (nraenv_ignores_env e2)
+      | NRAEnvMapConcat e1 e2 => (nraenv_ignores_env e1) /\ (nraenv_ignores_env e2)
+      | NRAEnvProduct e1 e2 => (nraenv_ignores_env e1) /\ (nraenv_ignores_env e2)
+      | NRAEnvSelect e1 e2 => (nraenv_ignores_env e1) /\ (nraenv_ignores_env e2)
+      | NRAEnvDefault e1 e2 => (nraenv_ignores_env e1) /\ (nraenv_ignores_env e2)
+      | NRAEnvEither e1 e2 => (nraenv_ignores_env e1) /\ (nraenv_ignores_env e2)
+      | NRAEnvEitherConcat e1 e2 => (nraenv_ignores_env e1) /\ (nraenv_ignores_env e2)
+      | NRAEnvApp e1 e2 => (nraenv_ignores_env e1) /\ (nraenv_ignores_env e2)
+      | NRAEnvGetConstant _ => True
+      | NRAEnvEnv => False
+      | NRAEnvAppEnv e1 e2 => (nraenv_ignores_env e2)
+      | NRAEnvMapEnv e1 => False
+      (* Those are additional operators *)
+      | NRAEnvFlatMap e1 e2 => (nraenv_ignores_env e1) /\ (nraenv_ignores_env e2)
+      | NRAEnvJoin e1 e2 e3 =>  (nraenv_ignores_env e1) /\ (nraenv_ignores_env e2) /\ (nraenv_ignores_env e3)
+      | NRAEnvProject _ e1 => (nraenv_ignores_env e1)
+      | NRAEnvGroupBy _ _ e1 => (nraenv_ignores_env e1)
+    end.
+
+  (* Java equivalent: NraOptimizer.nraenv_ignores_env_fun *)
+  Fixpoint nraenv_ignores_env_fun (e:nraenv) : bool :=
+    match e with
+      | NRAEnvID => true
+      | NRAEnvConst rd => true
+      | NRAEnvBinop bop e1 e2 => andb (nraenv_ignores_env_fun e1) (nraenv_ignores_env_fun e2)
+      | NRAEnvUnop uop e1 => nraenv_ignores_env_fun e1
+      | NRAEnvMap e1 e2 => andb (nraenv_ignores_env_fun e1) (nraenv_ignores_env_fun e2)
+      | NRAEnvMapConcat e1 e2 => andb (nraenv_ignores_env_fun e1) (nraenv_ignores_env_fun e2)
+      | NRAEnvProduct e1 e2 => andb (nraenv_ignores_env_fun e1) (nraenv_ignores_env_fun e2)
+      | NRAEnvSelect e1 e2 => andb (nraenv_ignores_env_fun e1) (nraenv_ignores_env_fun e2)
+      | NRAEnvDefault e1 e2 => andb (nraenv_ignores_env_fun e1) (nraenv_ignores_env_fun e2)
+      | NRAEnvEither e1 e2 => andb (nraenv_ignores_env_fun e1) (nraenv_ignores_env_fun e2)
+      | NRAEnvEitherConcat e1 e2 => andb (nraenv_ignores_env_fun e1) (nraenv_ignores_env_fun e2)
+      | NRAEnvApp e1 e2 => andb (nraenv_ignores_env_fun e1) (nraenv_ignores_env_fun e2)
+      | NRAEnvGetConstant _ => true
+      | NRAEnvEnv => false
+      | NRAEnvAppEnv e1 e2 => (nraenv_ignores_env_fun e2)
+      | NRAEnvMapEnv e1 => false
+      (* Those are additional operators *)
+      | NRAEnvFlatMap e1 e2 => andb (nraenv_ignores_env_fun e1) (nraenv_ignores_env_fun e2)
+      | NRAEnvJoin e1 e2 e3 =>  andb (nraenv_ignores_env_fun e1) (andb (nraenv_ignores_env_fun e2) (nraenv_ignores_env_fun e3))
+      | NRAEnvProject _ e1 => (nraenv_ignores_env_fun e1)
+      | NRAEnvGroupBy _ _ e1 => (nraenv_ignores_env_fun e1)
+    end.
+
+  Lemma nraenv_ignores_env_eq (e:nraenv):
+    nraenv_ignores_env e <-> (nraenv_ignores_env_fun e = true).
+  Proof.
+    induction e; split; simpl; intros; try auto; try congruence;
+    try (rewrite IHe1 in H; rewrite IHe2 in H;
+         elim H; clear H; intros;
+         rewrite H; rewrite H0; reflexivity);
+    try (rewrite andb_true_inversion in H;
+         elim H; clear H; intros;
+         rewrite <- IHe1 in H; rewrite <- IHe2 in H0;
+         split; assumption);
+    try (rewrite IHe in H; assumption);
+    try (rewrite <- IHe in H; assumption).
+    - rewrite <- IHe2; assumption.
+    - rewrite <- IHe2 in H; assumption.
+    - rewrite IHe1 in H; rewrite IHe2 in H; rewrite IHe3 in H.
+      elim H; clear H; intros.
+      elim H0; clear H0; intros.
+      rewrite H; rewrite H0; rewrite H1.
+      auto.
+    - rewrite andb_true_inversion in H.
+      rewrite andb_true_inversion in H.
+      elim H; clear H; intros.
+      elim H0; clear H0; intros.
+      rewrite <- IHe1 in H; rewrite <- IHe2 in H0; rewrite <- IHe3 in H1.
+      auto.
+  Qed.
+
+  (* Fixed environment ! *)
+
+  Fixpoint fixed_env (e:nraenv) : Prop :=
+    match e with
+      | NRAEnvID => True
+      | NRAEnvConst rd => True
+      | NRAEnvBinop bop e1 e2 => (fixed_env e1) /\ (fixed_env e2)
+      | NRAEnvUnop uop e1 => fixed_env e1
+      | NRAEnvMap e1 e2 => (fixed_env e1) /\ (fixed_env e2)
+      | NRAEnvMapConcat e1 e2 => (fixed_env e1) /\ (fixed_env e2)
+      | NRAEnvProduct e1 e2 => (fixed_env e1) /\ (fixed_env e2)
+      | NRAEnvSelect e1 e2 => (fixed_env e1) /\ (fixed_env e2)
+      | NRAEnvDefault e1 e2 => (fixed_env e1) /\ (fixed_env e2)
+      | NRAEnvEither e1 e2 => (fixed_env e1) /\ (fixed_env e2)
+      | NRAEnvEitherConcat e1 e2 => (fixed_env e1) /\ (fixed_env e2)
+      | NRAEnvApp e1 e2 => (fixed_env e1) /\ (fixed_env e2)
+      | NRAEnvGetConstant _ => True 
+      | NRAEnvEnv => True (* That's the difference with ignore... *)
+      | NRAEnvAppEnv e1 e2 => False (* Changes the environment *)
+      | NRAEnvMapEnv e1 => False (* Changes the environment *)
+      (* Those are additional operators *)
+      | NRAEnvFlatMap e1 e2 => (fixed_env e1) /\ (fixed_env e2)
+      | NRAEnvJoin e1 e2 e3 =>  (fixed_env e1) /\ (fixed_env e2) /\ (fixed_env e3)
+      | NRAEnvProject _ e1 => (fixed_env e1)
+      | NRAEnvGroupBy _ _ e1 => (fixed_env e1)
+    end.
+
+  Fixpoint fixed_env_fun (e:nraenv) : bool :=
+    match e with
+      | NRAEnvID => true
+      | NRAEnvConst rd => true
+      | NRAEnvBinop bop e1 e2 => andb (fixed_env_fun e1) (fixed_env_fun e2)
+      | NRAEnvUnop uop e1 => fixed_env_fun e1
+      | NRAEnvMap e1 e2 => andb (fixed_env_fun e1) (fixed_env_fun e2)
+      | NRAEnvMapConcat e1 e2 => andb (fixed_env_fun e1) (fixed_env_fun e2)
+      | NRAEnvProduct e1 e2 => andb (fixed_env_fun e1) (fixed_env_fun e2)
+      | NRAEnvSelect e1 e2 => andb (fixed_env_fun e1) (fixed_env_fun e2)
+      | NRAEnvDefault e1 e2 => andb (fixed_env_fun e1) (fixed_env_fun e2)
+      | NRAEnvEither e1 e2 => andb (fixed_env_fun e1) (fixed_env_fun e2)
+      | NRAEnvEitherConcat e1 e2 => andb (fixed_env_fun e1) (fixed_env_fun e2)
+      | NRAEnvApp e1 e2 => andb (fixed_env_fun e1) (fixed_env_fun e2)
+      | NRAEnvGetConstant _ => true
+      | NRAEnvEnv => true
+      | NRAEnvAppEnv e1 e2 => false
+      | NRAEnvMapEnv e1 => false
+      (* Those are additional operators *)
+      | NRAEnvFlatMap e1 e2 => andb (fixed_env_fun e1) (fixed_env_fun e2)
+      | NRAEnvJoin e1 e2 e3 =>  andb (fixed_env_fun e1) (andb (fixed_env_fun e2) (fixed_env_fun e3))
+      | NRAEnvProject _ e1 => (fixed_env_fun e1)
+      | NRAEnvGroupBy _ _ e1 => (fixed_env_fun e1)
+    end.
+
+  Lemma fixed_env_eq (e:nraenv):
+    fixed_env e <-> (fixed_env_fun e = true).
+  Proof.
+    induction e; split; simpl; intros; try auto; try congruence;
+    try (rewrite IHe1 in H; rewrite IHe2 in H;
+         elim H; clear H; intros;
+         rewrite H; rewrite H0; reflexivity);
+    try (rewrite andb_true_inversion in H;
+         elim H; clear H; intros;
+         rewrite <- IHe1 in H; rewrite <- IHe2 in H0;
+         split; assumption);
+    try (rewrite IHe in H; assumption);
+    try (rewrite <- IHe in H; assumption).
+    - rewrite IHe1 in H; rewrite IHe2 in H; rewrite IHe3 in H.
+      elim H; clear H; intros.
+      elim H0; clear H0; intros.
+      rewrite H; rewrite H0; rewrite H1.
+      auto.
+    - rewrite andb_true_inversion in H.
+      rewrite andb_true_inversion in H.
+      elim H; clear H; intros.
+      elim H0; clear H0; intros.
+      rewrite <- IHe1 in H; rewrite <- IHe2 in H0; rewrite <- IHe3 in H1.
+      auto.
+  Qed.
+
+  (* Nraenv_Ignores ID ... *)
+  
+  Fixpoint nraenv_ignores_id (e:nraenv) : Prop :=
+    match e with
+      | NRAEnvID => False
+      | NRAEnvConst rd => True
+      | NRAEnvBinop bop e1 e2 => (nraenv_ignores_id e1) /\ (nraenv_ignores_id e2)
+      | NRAEnvUnop uop e1 => nraenv_ignores_id e1
+      | NRAEnvMap e1 e2 => nraenv_ignores_id e2
+      | NRAEnvMapConcat e1 e2 => nraenv_ignores_id e2
+      | NRAEnvProduct e1 e2 => (nraenv_ignores_id e1) /\ (nraenv_ignores_id e2)
+      | NRAEnvSelect e1 e2 => (nraenv_ignores_id e2)
+      | NRAEnvDefault e1 e2 => (nraenv_ignores_id e1) /\ (nraenv_ignores_id e2)
+      | NRAEnvEither e1 e2 => False
+      | NRAEnvEitherConcat e1 e2 => (nraenv_ignores_id e1) /\ (nraenv_ignores_id e2)
+      | NRAEnvApp e1 e2 => (nraenv_ignores_id e2)
+      | NRAEnvGetConstant _ => True
+      | NRAEnvEnv => True
+      | NRAEnvAppEnv e1 e2 => (nraenv_ignores_id e1) /\ (nraenv_ignores_id e2)
+      | NRAEnvMapEnv e1 => (nraenv_ignores_id e1)
+      (* Those are additional operators *)
+      | NRAEnvFlatMap e1 e2 => (nraenv_ignores_id e1) /\ (nraenv_ignores_id e2)
+      | NRAEnvJoin e1 e2 e3 =>  (nraenv_ignores_id e1) /\ (nraenv_ignores_id e2) /\ (nraenv_ignores_id e3)
+      | NRAEnvProject _ e1 => (nraenv_ignores_id e1)
+      | NRAEnvGroupBy _ _ e1 => (nraenv_ignores_id e1)
+    end.
+
+  (* Java equivalent: NraOptimizer.nraenv_ignores_id_fun *)
+  Fixpoint nraenv_ignores_id_fun (e:nraenv) : bool :=
+    match e with
+      | NRAEnvID => false
+      | NRAEnvConst rd => true
+      | NRAEnvBinop bop e1 e2 => andb (nraenv_ignores_id_fun e1) (nraenv_ignores_id_fun e2)
+      | NRAEnvUnop uop e1 => nraenv_ignores_id_fun e1
+      | NRAEnvMap e1 e2 => nraenv_ignores_id_fun e2
+      | NRAEnvMapConcat e1 e2 => nraenv_ignores_id_fun e2
+      | NRAEnvProduct e1 e2 => andb (nraenv_ignores_id_fun e1) (nraenv_ignores_id_fun e2)
+      | NRAEnvSelect e1 e2 => (nraenv_ignores_id_fun e2)
+      | NRAEnvDefault e1 e2 => andb (nraenv_ignores_id_fun e1) (nraenv_ignores_id_fun e2)
+      | NRAEnvEither e1 e2 => false
+      | NRAEnvEitherConcat e1 e2 => andb (nraenv_ignores_id_fun e1) (nraenv_ignores_id_fun e2)
+      | NRAEnvApp e1 e2 => (nraenv_ignores_id_fun e2)
+      | NRAEnvGetConstant _ => true
+      | NRAEnvEnv => true
+      | NRAEnvAppEnv e1 e2 => andb (nraenv_ignores_id_fun e1) (nraenv_ignores_id_fun e2)
+      | NRAEnvMapEnv e1 => (nraenv_ignores_id_fun e1)
+      (* Those are additional operators *)
+      | NRAEnvFlatMap e1 e2 => andb (nraenv_ignores_id_fun e1) (nraenv_ignores_id_fun e2)
+      | NRAEnvJoin e1 e2 e3 =>  andb (nraenv_ignores_id_fun e1) (andb (nraenv_ignores_id_fun e2) (nraenv_ignores_id_fun e3))
+      | NRAEnvProject _ e1 => (nraenv_ignores_id_fun e1)
+      | NRAEnvGroupBy _ _ e1 => (nraenv_ignores_id_fun e1)
+    end.
+
+  Lemma nraenv_ignores_id_eq (e:nraenv):
+    nraenv_ignores_id e <-> (nraenv_ignores_id_fun e = true).
+  Proof.
+    induction e; split; simpl; intros; try auto; try congruence;
+    try (rewrite IHe1 in H; rewrite IHe2 in H;
+         elim H; clear H; intros;
+         rewrite H; rewrite H0; reflexivity);
+    try (rewrite andb_true_inversion in H;
+         elim H; clear H; intros;
+         rewrite <- IHe1 in H; rewrite <- IHe2 in H0;
+         split; assumption);
+    try (rewrite IHe in H; assumption);
+    try (rewrite <- IHe in H; assumption);
+    try (rewrite IHe2 in H; assumption);
+    try (rewrite <- IHe2 in H; assumption).
+    - rewrite IHe1 in H; rewrite IHe2 in H; rewrite IHe3 in H.
+      elim H; clear H; intros.
+      elim H0; clear H0; intros.
+      rewrite H; rewrite H0; rewrite H1.
+      auto.
+    - rewrite andb_true_inversion in H.
+      rewrite andb_true_inversion in H.
+      elim H; clear H; intros.
+      elim H0; clear H0; intros.
+      rewrite <- IHe1 in H; rewrite <- IHe2 in H0; rewrite <- IHe3 in H1.
+      auto.
+  Qed.
+
+  Require Import RAlgEnvIgnore.
+
+  Lemma nraenv_ignores_env_algenv_eq (e:nraenv) :
+    nraenv_ignores_env e ->
+    algenv_ignores_env (algenv_of_nraenv e).
+  Proof.
+    intros.
+    induction e; simpl in *; auto;
+    try (elim H; clear H; intros; auto).
+    - try (elim H0; clear H0; intros; auto).
+    - intuition.
+  Qed.
+  
+  Lemma nraenv_ignores_env_swap (e:nraenv) :
+    nraenv_ignores_env e -> forall (h:list (string*string)) c,
+                               forall (env1 env2:data), forall x:data,
+                       h ⊢ e @ₓ x ⊣ c;env1 = h ⊢ e @ₓ x ⊣ c;env2.
+  Proof.
+    intros.
+    unfold nraenv_eval.
+    apply algenv_ignores_env_swap.
+    apply nraenv_ignores_env_algenv_eq.
+    apply H.
+  Qed.
+  
+  Lemma nraenv_ignores_id_algenv_eq (e:nraenv) :
+    nraenv_ignores_id e ->
+    algenv_ignores_id (algenv_of_nraenv e).
+  Proof.
+    intros.
+    induction e; simpl in *; auto;
+    try (elim H; clear H; intros; auto).
+    - try (elim H0; clear H0; intros; auto).
+  Qed.
+  
+  Lemma nraenv_ignores_id_swap (e:nraenv) :
+    nraenv_ignores_id e -> forall h:list (string*string), forall c,
+      forall env:data, forall x1 x2:data,
+          h ⊢ e @ₓ x1 ⊣ c;env = h ⊢ e @ₓ x2 ⊣ c;env.
+  Proof.
+    intros.
+    unfold nraenv_eval.
+    apply algenv_ignores_id_swap.
+    apply nraenv_ignores_id_algenv_eq.
+    apply H.
+  Qed.
+
+End NRAEnvIgnore.
+
+(* 
+*** Local Variables: ***
+*** coq-load-path: (("../../../coq" "QCert")) ***
+*** End: ***
+*)
