coq/NRAEnv/Extended/NRAEnvSize.v
@@ -1,0 +1,87 @@
+(*
+ * Copyright 2015-2016 IBM Corporation
+ *
+ * Licensed under the Apache License, Version 2.0 (the "License");
+ * you may not use this file except in compliance with the License.
+ * You may obtain a copy of the License at
+ *
+ * http://www.apache.org/licenses/LICENSE-2.0
+ *
+ * Unless required by applicable law or agreed to in writing, software
+ * distributed under the License is distributed on an "AS IS" BASIS,
+ * WITHOUT WARRANTIES OR CONDITIONS OF ANY KIND, either express or implied.
+ * See the License for the specific language governing permissions and
+ * limitations under the License.
+ *)
+
+Section NRAEnvSize.
+  Require Import Omega.
+  Require Import BasicRuntime.
+  Require Import NRAEnv.
+
+  Context {fruntime:foreign_runtime}.
+
+  (* Java equivalent: NraOptimizer.optim_size.nraenv_size *)
+  Fixpoint nraenv_size (a:nraenv) : nat
+    := match a with
+         | NRAEnvID => 1
+         | NRAEnvConst d => 1
+         | NRAEnvBinop op a₁ a₂ => S (nraenv_size a₁ + nraenv_size a₂)
+         | NRAEnvUnop op a₁ => S (nraenv_size a₁)
+         | NRAEnvMap a₁ a₂ => S (nraenv_size a₁ + nraenv_size a₂)
+         | NRAEnvMapConcat a₁ a₂ => S (nraenv_size a₁ + nraenv_size a₂)
+         | NRAEnvProduct a₁ a₂ => S (nraenv_size a₁ + nraenv_size a₂)
+         | NRAEnvSelect a₁ a₂ => S (nraenv_size a₁ + nraenv_size a₂)
+         | NRAEnvDefault a₁ a₂ => S (nraenv_size a₁ + nraenv_size a₂)
+         | NRAEnvEither a₁ a₂ => S (nraenv_size a₁ + nraenv_size a₂)
+         | NRAEnvEitherConcat a₁ a₂ => S (nraenv_size a₁ + nraenv_size a₂)
+         | NRAEnvApp a₁ a₂ => S (nraenv_size a₁ + nraenv_size a₂)
+         | NRAEnvGetConstant _ => 1
+         | NRAEnvEnv => 1
+         | NRAEnvAppEnv a₁ a₂ => S (nraenv_size a₁ + nraenv_size a₂)
+         | NRAEnvMapEnv a₁ => S (nraenv_size a₁)
+         (* Those are additional operators *)
+         | NRAEnvFlatMap a₁ a₂ => S (nraenv_size a₁ + nraenv_size a₂)
+         | NRAEnvJoin a₁ a₂ a₃ => S (nraenv_size a₁ + nraenv_size a₂ + nraenv_size a₃)
+         | NRAEnvProject _ a₁ => S (nraenv_size a₁)
+         | NRAEnvGroupBy _ _ a₁ => S (nraenv_size a₁)
+       end.
+
+  Lemma nraenv_size_nzero (a:nraenv) : nraenv_size a <> 0.
+  Proof.
+    induction a; simpl; omega.
+  Qed.
+  
+  Fixpoint nraenv_depth (a:nraenv) : nat :=
+    (* Better to start at zero, level one is at least one nested plan *)
+    match a with
+    | NRAEnvID => 0
+    | NRAEnvConst d => 0
+    | NRAEnvBinop op a₁ a₂ => max (nraenv_depth a₁) (nraenv_depth a₂)
+    | NRAEnvUnop op a₁ => nraenv_depth a₁
+    | NRAEnvMap a₁ a₂ => max (S (nraenv_depth a₁)) (nraenv_depth a₂)
+    | NRAEnvMapConcat a₁ a₂ => max (S (nraenv_depth a₁)) (nraenv_depth a₂)
+    | NRAEnvProduct a₁ a₂ => max (nraenv_depth a₁) (nraenv_depth a₂)
+    | NRAEnvSelect a₁ a₂ => max (S (nraenv_depth a₁)) (nraenv_depth a₂)
+    | NRAEnvDefault a₁ a₂ => max (nraenv_depth a₁) (nraenv_depth a₂)
+    | NRAEnvEither a₁ a₂=> max (nraenv_depth a₁) (nraenv_depth a₂)
+    | NRAEnvEitherConcat a₁ a₂=> max (nraenv_depth a₁) (nraenv_depth a₂)
+    | NRAEnvApp a₁ a₂ => max (nraenv_depth a₁) (nraenv_depth a₂)
+    | NRAEnvGetConstant _ => 0
+    | NRAEnvEnv => 0
+    | NRAEnvAppEnv a₁ a₂ => max (nraenv_depth a₁) (nraenv_depth a₂)
+    | NRAEnvMapEnv a₁ => (S (nraenv_depth a₁))
+    (* Those are additional operators *)
+    | NRAEnvFlatMap a₁ a₂ => max (S (nraenv_depth a₁)) (nraenv_depth a₂)
+    | NRAEnvJoin a₁ a₂ a₃ => max (S (nraenv_depth a₁)) (max (nraenv_depth a₂) (nraenv_depth a₃))
+    | NRAEnvProject _ a₁ => (nraenv_size a₁)
+    | NRAEnvGroupBy _ _ a₁ => (nraenv_size a₁)
+    end.
+
+End NRAEnvSize.
+
+(* 
+*** Local Variables: ***
+*** coq-load-path: (("../../../coq" "QCert")) ***
+*** End: ***
+*)
